src/coq/dot/support.v
@@ -6,5 +6,13 @@ Ltac injsubst H := (injection H; intros; subst; clear H).
 
 Module lbl := LabelMapImpl.
 
+Tactic Notation "decls" "induction" ident(E) :=
+  try (intros until E);
+  let T := type of E in
+  let T := eval compute in T in
+  match T with
+    | list (label * ?A) => induction E using (lbl.alist_ind A)
+  end.
+
 Lemma binds_map_3 : forall A B l v (f: A -> B) args, lbl.binds l v ((lbl.map f) args) -> exists v', lbl.binds l v' args.
 Proof. Admitted.
